src/Compilers/Z/CommonSubexpressionEliminationInterp.v
@@ -1,0 +1,23 @@
+(** * Common Subexpression Elimination for PHOAS Syntax *)
+Require Import Coq.Lists.List.
+Require Import Crypto.Compilers.Syntax.
+Require Import Crypto.Compilers.Wf.
+Require Import Crypto.Compilers.Z.Syntax.
+Require Import Crypto.Compilers.CommonSubexpressionEliminationInterp.
+Require Import Crypto.Compilers.Z.CommonSubexpressionElimination.
+
+Lemma InterpCSE_gen t (e : Expr _ _ t) prefix
+      (Hwf : Wf e)
+  : forall x, Interp interp_op (@CSE_gen t e prefix) x = Interp interp_op e x.
+Proof.
+  apply InterpCSE;
+    auto using internal_base_type_dec_bl, internal_base_type_dec_lb, internal_symbolic_op_dec_bl, internal_symbolic_op_dec_lb, denote_symbolic_op.
+Qed.
+
+Lemma InterpCSE t (e : Expr _ _ t) (Hwf : Wf e)
+  : forall x, Interp interp_op (@CSE t e) x = Interp interp_op e x.
+Proof.
+  apply InterpCSE_gen; auto.
+Qed.
+
+Hint Rewrite @InterpCSE using solve_wf_side_condition : reflective_interp.
